Add mem_init_spec

theories/os/vmm.v
@@ -4,10 +4,27 @@ Require Import iris_os.os.page_table.
 Section vmm.
   Context `{clangG Σ} {pt: page_table Σ}.
 
-  Definition mem_init (n: int32) (x: addr) (y: addr) : expr :=
+  Definition mem_init (n: nat) (x: addr) (y: addr) : expr :=
     x <- Int.repr 0 ;;
-    while [ x :<: n ] ( x :<: n ) <{
+    while [ !x@Tint32 :<: Int.repr n ] ( !x@Tint32 :<: Int.repr n ) <{
       y <- Ealloc (Tprod Tint8 Tvoid) (Vpair vfalse Vvoid) ;;
-      insert_pt pt <$ Evalue (Vptr x) , Evalue (Vptr y) $>
+      insert_pt pt <$ !x@Tint32 , Evalue (Vptr y) $>
     }>.
+
+  Fixpoint allocated m (n: nat) : iProp Σ :=
+    match m !! Int.repr n with
+      | None => False%I
+      | Some p =>
+        (p ↦ (Vpair vfalse Vvoid) @ (Tprod Tint8 Tvoid) ∗
+           match n with
+             | O => True
+             | S n' => allocated m n'
+        end)%I
+      end.
+
+  Lemma mem_init_spec n x y Φ:
+    is_page_table pt ∅ ∗ (∀ m, allocated m (n - 1) -∗ is_page_table pt m -∗ Φ Vvoid)
+    ⊢ WP mem_init n x y {{ Φ }}.
+  Admitted.
+
 End vmm.
